Logical Relation + beginning FTLR

theories/ftlr/ftlr_base.v
@@ -15,35 +15,31 @@ Section fundamental.
   
 
   Definition ftlr_instr (r : leibnizO Reg) (p : Perm)
-        (b e a : Addr) (w : Word) (i: instr) (P : D) := 
+        (b e a : Addr) (w : Word) (it: instr) (i : CoreN) (P : D) :=
       p = RX ∨ p = RWX
-    → (∀ x : RegName, is_Some (r !! x))
+    → (∀ x : RegName, is_Some (r !! (i, x)))
     → isCorrectPC (WCap p b e a)
     → (b <= a)%a ∧ (a < e)%a
-    → decodeInstrW w = i
+    → decodeInstrW w = it
     -> □ ▷ (∀ a0 a1 a2 a3 a4,
-             full_map a0
-          -∗ (∀ (r1 : RegName) v, ⌜r1 ≠ PC⌝ → ⌜a0 !! r1 = Some v⌝ → (fixpoint interp1) v)
-          -∗ registers_mapsto (<[PC:=WCap a1 a2 a3 a4]> a0)
-          -∗ na_own logrel_nais ⊤
-             -∗ □ (fixpoint interp1) (WCap a1 a2 a3 a4) -∗ interp_conf)
+             full_map a0 i
+          -∗ (∀ (j : CoreN) (r1 : RegName) v, ⌜r1 ≠ PC⌝ → ⌜a0 !! (j, r1) = Some v⌝ → (fixpoint interp1) v)
+          -∗ registers_mapsto (<[(i, PC):=WCap a1 a2 a3 a4]> a0)
+             -∗ □ (fixpoint interp1) (WCap a1 a2 a3 a4) -∗ (interp_conf i))
     -∗ (fixpoint interp1) (WCap p b e a)
     -∗ inv (logN.@a) (∃ w0 : leibnizO Word, a ↦ₐ w0 ∗ P w0)
-    -∗ (∀ (r1 : RegName) v, ⌜r1 ≠ PC⌝ → ⌜r !! r1 = Some v⌝ → (fixpoint interp1) v)
+    -∗ (∀ (j : CoreN) (r1 : RegName) v, ⌜r1 ≠ PC⌝ → ⌜r !! (j, r1) = Some v⌝ → (fixpoint interp1) v)
     -∗ ▷ □ (∀ w : Word, P w -∗ (fixpoint interp1) w)
-            ∗ (if decide (writeAllowed_in_r_a (<[PC:=WCap p b e a]> r) a) then ▷ □ (∀ w : Word, (fixpoint interp1) w -∗ P w) else emp)
-    -∗ na_own logrel_nais ⊤
+            ∗ (if decide (writeAllowed_in_r_a (<[(i, PC):=WCap p b e a]> r) i a) then ▷ □ (∀ w : Word, (fixpoint interp1) w -∗ P w) else emp)
     -∗ a ↦ₐ w
     -∗ ▷ P w
     -∗ (▷ (∃ w0 : leibnizO Word, a ↦ₐ w0 ∗ P w0) ={⊤ ∖ ↑logN.@a,⊤}=∗ emp)
-    -∗ PC ↦ᵣ WCap p b e a
-    -∗ ([∗ map] k↦y ∈ delete PC (<[PC:=WCap p b e a]> r), k ↦ᵣ y)
+    -∗ (i, PC) ↦ᵣ WCap p b e a
+    -∗ ([∗ map] k↦y ∈ delete (i, PC) (<[(i, PC):=WCap p b e a]> r), k ↦ᵣ y)
     -∗
-        WP Instr Executable
-        @ ⊤ ∖ ↑logN.@a {{ v, |={⊤ ∖ ↑logN.@a,⊤}=> WP Seq (of_val v)
-                                                    {{ v0, ⌜v0 = HaltedV⌝
-                                                           → ∃ r1 : Reg, full_map r1 ∧ registers_mapsto r1
-                                                                                                        ∗ na_own logrel_nais ⊤ }} }}.
-
-
+        WP (i, Instr Executable)
+        @ ⊤ ∖ ↑logN.@a {{ v, |={⊤ ∖ ↑logN.@a,⊤}=> WP fill_item SeqCtx (of_val v)
+                                                    {{ v0, ⌜v0 = (i, HaltedV)⌝
+                                                           → ∃ r1 : Reg
+                                                          , full_map r1 i ∧ registers_mapsto r1}} }}.
 End fundamental.
