theories/ftlr/Get.v
@@ -15,36 +15,43 @@ Section fundamental.
   Implicit Types interp : (D).
 
   Lemma get_case (r : leibnizO Reg) (p : Perm)
-        (b e a : Addr) (w : Word) (dst r0 : RegName) (ins: instr) (P:D) :
+        (b e a : Addr) (w : Word) (dst r0 : RegName) (ins: instr) (i : CoreN) (P:D) :
     is_Get ins dst r0 →
-    ftlr_instr r p b e a w ins P.
+    ftlr_instr r p b e a w ins i P.
   Proof.
-    intros Hinstr Hp Hsome i Hbae Hi.
-    iIntros "#IH #Hinv #Hinva #Hreg #[Hread Hwrite] Hown Ha HP Hcls HPC Hmap".
+    intros Hinstr Hp Hsome i' Hbae Hi.
+    iIntros "#IH #Hinv #Hinva #Hreg #[Hread Hwrite] Ha HP Hcls HPC Hmap".
     rewrite delete_insert_delete.
     rewrite <- Hi in Hinstr. clear Hi.
-    iDestruct ((big_sepM_delete _ _ PC) with "[HPC Hmap]") as "Hmap /=";
+    iDestruct ((big_sepM_delete _ _ (i, PC)) with "[HPC Hmap]") as "Hmap /=";
       [apply lookup_insert|rewrite delete_insert_delete;iFrame|]. simpl.
     iApply (wp_Get with "[$Ha $Hmap]"); eauto.
     { simplify_map_eq; auto. }
-    { rewrite /subseteq /map_subseteq /set_subseteq_instance. intros rr _.
-      apply elem_of_gmap_dom. apply lookup_insert_is_Some'; eauto. }
-
+    { rewrite /regs_of_core /subseteq /map_subseteq /set_subseteq_instance. intros rr ?.
+      apply elem_of_gmap_dom. apply lookup_insert_is_Some'; eauto.
+      set_solver.
+    }
     iIntros "!>" (regs' retv). iDestruct 1 as (HSpec) "[Ha Hmap]".
     destruct HSpec; cycle 1.
     { iApply wp_pure_step_later; auto. iMod ("Hcls" with "[HP Ha]");[iExists w;iFrame|iModIntro]. iNext.
-      iApply wp_value; auto. iIntros; discriminate. }
+      iApply wp_value; auto. } (* iIntros ; discriminate. } *)
     { incrementPC_inv; simplify_map_eq.
       iApply wp_pure_step_later; auto. iMod ("Hcls" with "[HP Ha]");[iExists w;iFrame|iModIntro]. iNext.
       assert (dst <> PC) as HdstPC by (intros ->; simplify_map_eq).
       simplify_map_eq.
-      iApply ("IH" $! (<[dst := _]> (<[PC := _]> r)) with "[%] [] [Hmap] [$Hown]");
+      iApply ("IH" $! (<[(i, dst) := _]> (<[(i, PC) := _]> r)) with "[%] [] [Hmap]");
         try iClear "IH"; eauto.
       { intro. cbn. by repeat (rewrite lookup_insert_is_Some'; right). }
-      iIntros (ri v Hri Hsv). rewrite insert_commute // lookup_insert_ne // in Hsv; [].
-      destruct (decide (ri = dst)); simplify_map_eq.
+      iIntros (j ri v Hri Hsv).
+      rewrite insert_commute in Hsv ;[| simplify_pair_eq].
+      rewrite lookup_insert_ne in Hsv ;[| simplify_pair_eq].
+      destruct (decide ((j, ri) = (i,dst))); simplify_map_eq.
       { repeat rewrite fixpoint_interp1_eq; auto. }
-      { by iApply "Hreg". } rewrite !fixpoint_interp1_eq /=. destruct Hp as [-> | ->];iFrame "Hinv". }
+      { iApply "Hreg". done. iPureIntro. eauto. }
+      rewrite lookup_insert_ne in H1
+      ;[| simplify_pair_eq] ; simplify_map_eq.
+      rewrite !fixpoint_interp1_eq /=.
+      destruct Hp as [-> | ->]; iFrame "Hinv". }
   Qed.
 
 End fundamental.
