theories/ftlr/Jmp.v
@@ -17,11 +17,11 @@ Section fundamental.
 
 
   Lemma jmp_case (r : leibnizO Reg) (p : Perm)
-        (b e a : Addr) (w : Word) (r0 : RegName) (P : D):
-    ftlr_instr r p b e a w (Jmp r0) P.
+        (b e a : Addr) (w : Word) (r0 : RegName) (i : CoreN) (P : D):
+    ftlr_instr r p b e a w (Jmp r0) i P.
   Proof.
-    intros Hp Hsome i Hbae Hi.
-    iIntros "#IH #Hinv #Hinva #Hreg #Hread Hown Ha HP Hcls HPC Hmap".
+    intros Hp Hsome i' Hbae Hi.
+    iIntros "#IH #Hinv #Hinva #Hreg #Hread Ha HP Hcls HPC Hmap".
     rewrite delete_insert_delete.
     destruct (reg_eq_dec PC r0).
     * subst r0.
@@ -33,25 +33,25 @@ Section fundamental.
       iApply wp_pure_step_later; auto.
       (* reconstruct registers *)
       iNext. 
-      iDestruct ((big_sepM_delete _ _ PC) with "[HPC Hmap]") as "Hmap /=";
+      iDestruct ((big_sepM_delete _ _ (i, PC)) with "[HPC Hmap]") as "Hmap /=";
         [apply lookup_insert|rewrite delete_insert_delete;iFrame|]. simpl.
       (* apply IH *)
-      iApply ("IH" $! _ _ b e a with "[] [] [Hmap] [$Hown]"); eauto.
+      iApply ("IH" $! _ _ b e a with "[] [] [Hmap]"); eauto.
       { iPureIntro. apply Hsome. }
       destruct Hp as [-> | ->]; iFrame.
     * specialize Hsome with r0 as Hr0.
       destruct Hr0 as [wsrc Hsomesrc].
-      iDestruct ((big_sepM_delete _ _ r0) with "Hmap") as "[Hsrc Hmap]"; eauto.
-      rewrite (lookup_delete_ne r PC r0); eauto.
+      iDestruct ((big_sepM_delete _ _ (i, r0)) with "Hmap") as "[Hsrc Hmap]"; eauto.
+      rewrite (lookup_delete_ne r (i, PC) (i, r0)) ; eauto ; simplify_pair_eq.
       iApply (wp_jmp_success with "[$HPC $Ha $Hsrc]"); eauto.
       iNext. iIntros "[HPC [Ha Hsrc]] /=".
       iApply wp_pure_step_later; auto. 
       (* reconstruct regions *)
-      iDestruct ((big_sepM_delete _ _ r0) with "[Hsrc Hmap]") as "Hmap /=";
+      iDestruct ((big_sepM_delete _ _ (i, r0)) with "[Hsrc Hmap]") as "Hmap /=";
         [apply lookup_insert|rewrite delete_insert_delete;iFrame|]. simpl.
       rewrite -delete_insert_ne; auto. 
       destruct (updatePcPerm wsrc) eqn:Heq.
-      { iApply (wp_bind (fill [SeqCtx])).
+      { iApply (wp_bind (fill [SeqCtx]) _ _ (_, _) _).
         iApply (wp_notCorrectPC with "HPC"); [intro; match goal with H: isCorrectPC (WInt _) |- _ => inv H end|].
         iMod ("Hcls" with "[Ha HP]") as "_";[iExists w; iFrame|].
         iModIntro. 
@@ -60,7 +60,7 @@ Section fundamental.
         iApply wp_value.
         iNext. iIntros. discriminate. }
       { destruct p0.
-        - iApply (wp_bind (fill [SeqCtx])).
+        - iApply (wp_bind (fill [SeqCtx]) _ _ (_,_) _).
           iApply (wp_notCorrectPC with "HPC"); [eapply not_isCorrectPC_perm; eauto|].
           iMod ("Hcls" with "[Ha HP]") as "_";[iExists w; iFrame|].
           iModIntro. 
@@ -68,7 +68,7 @@ Section fundamental.
           iApply wp_pure_step_later; auto.
           iApply wp_value.
           iNext. iIntros. discriminate.
-        - iApply (wp_bind (fill [SeqCtx])).
+        - iApply (wp_bind (fill [SeqCtx]) _ _ (_,_) _).
           iApply (wp_notCorrectPC with "HPC"); [eapply not_isCorrectPC_perm; eauto|].
           iMod ("Hcls" with "[Ha HP]") as "_";[iExists w; iFrame|].
           iModIntro. 
@@ -76,7 +76,7 @@ Section fundamental.
           iApply wp_pure_step_later; auto.
           iApply wp_value.
           iNext. iIntros. discriminate.
-        - iApply (wp_bind (fill [SeqCtx])).
+        - iApply (wp_bind (fill [SeqCtx]) _ _ (_,_) _).
           iApply (wp_notCorrectPC with "HPC"); [eapply not_isCorrectPC_perm; eauto|].
           iMod ("Hcls" with "[Ha HP]") as "_";[iExists w; iFrame|].
           iModIntro. 
@@ -84,44 +84,46 @@ Section fundamental.
           iApply wp_pure_step_later; auto.
           iApply wp_value.
           iNext. iIntros. discriminate.
-        - iDestruct ((big_sepM_delete _ _ PC) with "[HPC Hmap]") as "Hmap /=".
+        - iDestruct ((big_sepM_delete _ _ (i, PC)) with "[HPC Hmap]") as "Hmap /=".
           apply lookup_insert. rewrite delete_insert_delete. iFrame.
-          rewrite (insert_id r r0); auto.
-          iDestruct ("Hreg" $! r0 _ _ Hsomesrc) as "Hwsrc".
+          rewrite (insert_id r (i, r0)); auto.
+          iDestruct ("Hreg" $! i r0 _ _ Hsomesrc) as "Hwsrc".
           destruct wsrc; simpl in Heq; try congruence.
           destruct p0; try congruence.
           + iMod ("Hcls" with "[Ha HP]") as "_";[iExists w; iFrame|].
             iModIntro. 
             inv Heq.
             iNext.
-            iApply ("IH" with "[] [] [$Hmap] [$Hown]"); eauto.
+            iApply ("IH" with "[] [] [$Hmap]"); eauto.
           + inv Heq.
             rewrite /interp_expr /=.
             iDestruct "Hwsrc" as "#H".
             iMod ("Hcls" with "[Ha HP]") as "_";[iExists w; iFrame|].
             iModIntro.
-            rewrite !fixpoint_interp1_eq /=. iDestruct ("H" with "[$Hmap $Hown]") as "Hcont"; auto.
-        - iApply (wp_bind (fill [SeqCtx])).
+            rewrite !fixpoint_interp1_eq /=. iDestruct ("H" with "[$Hmap]") as
+              "Hcont"; auto.
+        - iApply (wp_bind (fill [SeqCtx]) _ _ (_,_) _).
           iApply (wp_notCorrectPC with "HPC"); [eapply not_isCorrectPC_perm; eauto|].
           iMod ("Hcls" with "[Ha HP]") as "_";[iExists w; iFrame|].
           iModIntro.
           iNext. iNext. iIntros "HPC /=".
           iApply wp_pure_step_later; auto.
           iApply wp_value.
-          iNext. iIntros. discriminate.
+          iNext. iIntros.
+          discriminate.
         - iMod ("Hcls" with "[Ha HP]") as "_";[iExists w; iFrame|].
           iModIntro.
           iNext.
-          iDestruct ((big_sepM_delete _ _ PC) with "[HPC Hmap]") as "Hmap /=".
+          iDestruct ((big_sepM_delete _ _ (i, PC)) with "[HPC Hmap]") as "Hmap /=".
           apply lookup_insert. rewrite delete_insert_delete. iFrame.
-          rewrite (insert_id r r0); auto.
+          rewrite (insert_id r (i, r0)); auto.
           destruct wsrc; simpl in Heq; try congruence.
           destruct p0; try congruence. inv Heq.
-          iDestruct ("Hreg" $! r0 _ _ Hsomesrc) as "Hwsrc".
+          iDestruct ("Hreg" $! i r0 _ _ Hsomesrc) as "Hwsrc".
           iClear "Hinv".
-          iApply ("IH" with "[] [] [Hmap] [$Hown]"); iFrame "#"; eauto.
+          iApply ("IH" with "[] [] [Hmap]"); iFrame "#"; eauto.
       }
-      Unshelve. all: auto.
+      Unshelve. all: auto ; simplify_pair_eq.
   Qed.
   
 End fundamental.
