theories/fundamental.v
@@ -1,4 +1,5 @@
-From cap_machine.ftlr Require Export Jmp Jnz Mov Load Store AddSubLt Restrict Subseg IsPtr Get Lea. 
+(* From cap_machine.ftlr Require Export Jmp Jnz Mov Load Store AddSubLt Restrict Subseg IsPtr Get Lea.  *)
+From cap_machine.ftlr Require Export Jmp Get.
 From iris.proofmode Require Import tactics.
 From iris.program_logic Require Import weakestpre adequacy lifting.
 From stdpp Require Import base.
@@ -6,7 +7,6 @@ From cap_machine Require Export logrel.
 
 Section fundamental.
   Context {Σ:gFunctors} {memg:memG Σ} {regg:regG Σ}
-          {nainv: logrel_na_invs Σ}
           `{MP: MachineParameters}.
 
   Notation D := ((leibnizO Word) -n> iPropO Σ).
@@ -14,99 +14,110 @@ Section fundamental.
   Implicit Types w : (leibnizO Word).
   Implicit Types interp : (D).
 
-  Lemma extract_r_ex r (reg : RegName) :
-    (∃ w, r !! reg = Some w) →
-    ⊢ (([∗ map] r0↦w ∈ r, r0 ↦ᵣ w) → ∃ w, reg ↦ᵣ w)%I.
+  Lemma extract_r_ex r i (reg : RegName) :
+    (∃ w, r !! (i, reg) = Some w) →
+    ⊢ (([∗ map] r0↦w ∈ r, r0 ↦ᵣ w) → ∃ w, (i, reg) ↦ᵣ w)%I.
   Proof.
     intros [w Hw].
     iIntros "Hmap". iExists w. 
-    iApply (big_sepM_lookup (λ reg' i, reg' ↦ᵣ i)%I r reg w); eauto. 
+    iApply (big_sepM_lookup (λ reg' j, reg' ↦ᵣ j)%I r (i, reg) w); eauto.
   Qed.
 
-  Lemma extract_r reg (r : RegName) w :
-    reg !! r = Some w →
+  Lemma extract_r reg i (r : RegName) w :
+    reg !! (i, r) = Some w →
     ⊢ (([∗ map] r0↦w ∈ reg, r0 ↦ᵣ w) →
-     (r ↦ᵣ w ∗ (∀ x', r ↦ᵣ x' -∗ [∗ map] k↦y ∈ <[r := x']> reg, k ↦ᵣ y)))%I.
+     ((i, r) ↦ᵣ w ∗ (∀ x', (i, r) ↦ᵣ x' -∗ [∗ map] k↦y ∈ <[(i, r) := x']> reg, k ↦ᵣ y)))%I.
   Proof.
     iIntros (Hw) "Hmap". 
-    iDestruct (big_sepM_lookup_acc (λ (r : RegName) i, r ↦ᵣ i)%I reg r w) as "Hr"; eauto.
+    iDestruct (big_sepM_lookup_acc (λ k j, k ↦ᵣ j)%I reg (i, r) w) as "Hr"; eauto.
     iSpecialize ("Hr" with "[Hmap]"); eauto. iDestruct "Hr" as "[Hw Hmap]".
-    iDestruct (big_sepM_insert_acc (λ (r : RegName) i, r ↦ᵣ i)%I reg r w) as "Hupdate"; eauto.
+    iDestruct (big_sepM_insert_acc (λ k j, k ↦ᵣ j)%I reg (i, r) w) as "Hupdate"; eauto.
     iSpecialize ("Hmap" with "[Hw]"); eauto. 
     iSpecialize ("Hupdate" with "[Hmap]"); eauto.
   Qed.
   
-  Lemma fundamental_cap r p b e a :
+  Lemma fundamental_cap i r p b e a :
     ⊢ interp (WCap p b e a) →
-      interp_expression r (WCap p b e a).
+      interp_expression r i (WCap p b e a).
   Proof.
     iIntros "#Hinv /=".
-    iIntros "[[Hfull Hreg] [Hmreg Hown]]".
+    iIntros "[[Hfull Hreg] Hmreg]".
     iRevert "Hinv".
     iLöb as "IH" forall (r p b e a).
     iIntros "#Hinv". 
-    iDestruct "Hfull" as "%". iDestruct "Hreg" as "#Hreg". 
-    iApply (wp_bind (fill [SeqCtx])).
+    iDestruct "Hfull" as "%". iDestruct "Hreg" as "#Hreg".
+    iApply (wp_bind (fill [SeqCtx]) _ _ (_, _) _).
     destruct (decide (isCorrectPC (WCap p b e a))).
     - (* Correct PC *)
       assert ((b <= a)%a ∧ (a < e)%a) as Hbae.
       { eapply in_range_is_correctPC; eauto. solve_addr. }
       assert (p = RX ∨ p = RWX) as Hp.
-      { inversion i. subst. auto. }
+      { inversion i0. subst. auto. }
       iDestruct (read_allowed_inv_regs with "[] Hinv") as (P) "(#Hinva & #Hread)";[eauto|destruct Hp as [-> | ->];auto|iFrame "% #"|].
       rewrite /interp_ref_inv /=. 
       iInv (logN.@a) as (w) "[>Ha HP]" "Hcls". 
-      iDestruct ((big_sepM_delete _ _ PC) with "Hmreg") as "[HPC Hmap]"; 
+      iDestruct ((big_sepM_delete _ _ (i, PC)) with "Hmreg") as "[HPC Hmap]";
         first apply (lookup_insert _ _ (WCap p b e a)).
       destruct (decodeInstrW w) eqn:Hi. (* proof by cases on each instruction *)
       + (* Jmp *)
-        iApply (jmp_case with "[] [] [] [] [] [Hown] [Ha] [HP] [Hcls] [HPC] [Hmap]");
-          try iAssumption; eauto. 
-      + (* Jnz *)
-        iApply (jnz_case with "[] [] [] [] [] [Hown] [Ha] [HP] [Hcls] [HPC] [Hmap]");
-          try iAssumption; eauto.
-      + (* Mov *)
-        iApply (mov_case with "[] [] [] [] [] [Hown] [Ha] [HP] [Hcls] [HPC] [Hmap]");
-          try iAssumption; eauto.
-      + (* Load *)
-        iApply (load_case with "[] [] [] [] [] [Hown] [Ha] [HP] [Hcls] [HPC] [Hmap]");
-          try iAssumption; eauto.
-      + (* Store *)
-        iApply (store_case with "[] [] [] [] [] [Hown] [Ha] [HP] [Hcls] [HPC] [Hmap]");
-          try iAssumption; eauto.
-      + (* Lt *)
-        iApply (add_sub_lt_case with "[] [] [] [] [] [Hown] [Ha] [HP] [Hcls] [HPC] [Hmap]");
-          try iAssumption; eauto.
-      + (* Add *)
-        iApply (add_sub_lt_case with "[] [] [] [] [] [Hown] [Ha] [HP] [Hcls] [HPC] [Hmap]");
-          try iAssumption; eauto.
-      + (* Sub *)
-        iApply (add_sub_lt_case with "[] [] [] [] [] [Hown] [Ha] [HP] [Hcls] [HPC] [Hmap]");
-          try iAssumption; eauto.
-      + (* Lea *)
-        iApply (lea_case with "[] [] [] [] [] [Hown] [Ha] [HP] [Hcls] [HPC] [Hmap]");
-          try iAssumption; eauto.
-      + (* Restrict *)
-        iApply (restrict_case with "[] [] [] [] [] [Hown] [Ha] [HP] [Hcls] [HPC] [Hmap]");
-          try iAssumption; eauto.
-      + (* Subseg *)
-        iApply (subseg_case with "[] [] [] [] [] [Hown] [Ha] [HP] [Hcls] [HPC] [Hmap]");
-          try iAssumption; eauto.
-      + (* IsPtr *)
-        iApply (isptr_case with "[] [] [] [] [] [Hown] [Ha] [HP] [Hcls] [HPC] [Hmap]");
-          try iAssumption; eauto.
+        iApply (jmp_case with "[] [] [] [] [] [Ha] [HP] [Hcls] [HPC] [Hmap]");
+          try iAssumption; eauto ; iFrame "Hread".
+      + admit.
+      + admit.
+      + admit.
+      + admit.
+      + admit.
+      + admit.
+      + admit.
+      + admit.
+      + admit.
+      + admit.
+      + admit.
+      (* + (* Jnz *) *)
+      (*   iApply (jnz_case with "[] [] [] [] [] [Ha] [HP] [Hcls] [HPC] [Hmap]"); *)
+      (*     try iAssumption; eauto. *)
+      (* + (* Mov *) *)
+      (*   iApply (mov_case with "[] [] [] [] [] [Ha] [HP] [Hcls] [HPC] [Hmap]"); *)
+      (*     try iAssumption; eauto. *)
+      (* + (* Load *) *)
+      (*   iApply (load_case with "[] [] [] [] [] [Ha] [HP] [Hcls] [HPC] [Hmap]"); *)
+      (*     try iAssumption; eauto. *)
+      (* + (* Store *) *)
+      (*   iApply (store_case with "[] [] [] [] [] [Ha] [HP] [Hcls] [HPC] [Hmap]"); *)
+      (*     try iAssumption; eauto. *)
+      (* + (* Lt *) *)
+      (*   iApply (add_sub_lt_case with "[] [] [] [] [] [Ha] [HP] [Hcls] [HPC] [Hmap]"); *)
+      (*     try iAssumption; eauto. *)
+      (* + (* Add *) *)
+      (*   iApply (add_sub_lt_case with "[] [] [] [] [] [Ha] [HP] [Hcls] [HPC] [Hmap]"); *)
+      (*     try iAssumption; eauto. *)
+      (* + (* Sub *) *)
+      (*   iApply (add_sub_lt_case with "[] [] [] [] [] [Ha] [HP] [Hcls] [HPC] [Hmap]"); *)
+      (*     try iAssumption; eauto. *)
+      (* + (* Lea *) *)
+      (*   iApply (lea_case with "[] [] [] [] [] [Ha] [HP] [Hcls] [HPC] [Hmap]"); *)
+      (*     try iAssumption; eauto. *)
+      (* + (* Restrict *) *)
+      (*   iApply (restrict_case with "[] [] [] [] [] [Ha] [HP] [Hcls] [HPC] [Hmap]"); *)
+      (*     try iAssumption; eauto. *)
+      (* + (* Subseg *) *)
+      (*   iApply (subseg_case with "[] [] [] [] [] [Ha] [HP] [Hcls] [HPC] [Hmap]"); *)
+      (*     try iAssumption; eauto. *)
+      (* + (* IsPtr *) *)
+      (*   iApply (isptr_case with "[] [] [] [] [] [Ha] [HP] [Hcls] [HPC] [Hmap]"); *)
+      (*     try iAssumption; eauto. *)
       + (* GetP *)
-        iApply (get_case _ _ _ _ _ _ _ _ (GetP _ _) with "[] [] [] [] [] [Hown] [Ha] [HP] [Hcls] [HPC] [Hmap]");
-          try iAssumption; eauto.
+        iApply (get_case _ _ _ _ _ _ _ _ (GetP _ _) with "[] [] [] [] [] [Ha] [HP] [Hcls] [HPC] [Hmap]");
+          try iAssumption; eauto ; iFrame "Hread".
       + (* GetB *)
-        iApply (get_case _ _ _ _ _ _ _ _ (GetB _ _) with "[] [] [] [] [] [Hown] [Ha] [HP] [Hcls] [HPC] [Hmap]");
-          try iAssumption; eauto.
+        iApply (get_case _ _ _ _ _ _ _ _ (GetB _ _) with "[] [] [] [] [] [Ha] [HP] [Hcls] [HPC] [Hmap]");
+          try iAssumption; eauto ; iFrame "Hread".
       + (* GetE *)
-        iApply (get_case _ _ _ _ _ _ _ _ (GetE _ _) with "[] [] [] [] [] [Hown] [Ha] [HP] [Hcls] [HPC] [Hmap]");
-          try iAssumption; eauto.
+        iApply (get_case _ _ _ _ _ _ _ _ (GetE _ _) with "[] [] [] [] [] [Ha] [HP] [Hcls] [HPC] [Hmap]");
+          try iAssumption; eauto ; iFrame "Hread".
       + (* GetA *)
-        iApply (get_case _ _ _ _ _ _ _ _ (GetA _ _) with "[] [] [] [] [] [Hown] [Ha] [HP] [Hcls] [HPC] [Hmap]");
-          try iAssumption; eauto.
+        iApply (get_case _ _ _ _ _ _ _ _ (GetA _ _) with "[] [] [] [] [] [Ha] [HP] [Hcls] [HPC] [Hmap]");
+          try iAssumption; eauto ; iFrame "Hread".
       + (* Fail *)
         iApply (wp_fail with "[HPC Ha]"); eauto; iFrame.
         iNext. iIntros "[HPC Ha] /=".
@@ -120,32 +131,32 @@ Section fundamental.
         iMod ("Hcls" with "[HP Ha]");[iExists w;iFrame|iModIntro].
         iApply wp_pure_step_later; auto.
         iApply wp_value.
-        iDestruct ((big_sepM_delete _ _ PC) with "[HPC Hmap]") as "Hmap /=".
+        iDestruct ((big_sepM_delete _ _ (i, PC)) with "[HPC Hmap]") as "Hmap /=".
         apply lookup_insert. rewrite delete_insert_delete. iFrame.
         rewrite insert_insert. iNext. iIntros (_). 
-        iExists (<[PC:=WCap p b e a]> r). iFrame.
-        iAssert (∀ r0 : RegName, ⌜is_Some (<[PC:=WCap p b e a]> r !! r0)⌝)%I as "HA".
+        iExists (<[(i, PC):=WCap p b e a]> r). iFrame.
+        iAssert (∀ r0 : RegName, ⌜is_Some (<[(i, PC):=WCap p b e a]> r !! (i, r0))⌝)%I as "HA".
         { iIntros. destruct (reg_eq_dec PC r0).
           - subst r0; rewrite lookup_insert; eauto.
-          - rewrite lookup_insert_ne; auto. }
+          - rewrite lookup_insert_ne; auto ; simplify_pair_eq. }
         iFrame "HA".
    - (* Not correct PC *)
-     iDestruct ((big_sepM_delete _ _ PC) with "Hmreg") as "[HPC Hmap]";
+     iDestruct ((big_sepM_delete _ _ (i, PC)) with "Hmreg") as "[HPC Hmap]";
        first apply (lookup_insert _ _ (WCap p b e a)).
      iApply (wp_notCorrectPC with "HPC"); eauto.
      iNext. iIntros "HPC /=".
      iApply wp_pure_step_later; auto.
      iApply wp_value.
      iNext. iIntros (Hcontr); inversion Hcontr.
-  Qed.
+  Admitted.
 
-  Theorem fundamental w r :
-    ⊢ interp w -∗ interp_expression r w.
+  Theorem fundamental i w r :
+    ⊢ interp w -∗ interp_expression i r w.
   Proof.
     iIntros "Hw". destruct w as [| c].
-    { iClear "Hw". iIntros "(? & Hreg & ?)". unfold interp_conf.
+    { iClear "Hw". iIntros "(? & Hreg)". unfold interp_conf.
       iApply (wp_wand with "[-]"). 2: iIntros (?) "H"; iApply "H".
-      iApply (wp_bind (fill [SeqCtx])). cbn.
+      iApply (wp_bind (fill [SeqCtx]) _ _ (_,_)). cbn.
       unfold registers_mapsto. rewrite -insert_delete.
       iDestruct (big_sepM_insert with "Hreg") as "[HPC ?]". by rewrite lookup_delete.
       iApply (wp_notCorrectPC with "HPC"). by inversion 1.
@@ -157,13 +168,13 @@ Section fundamental.
   (* The fundamental theorem implies the exec_cond *)
 
   Definition exec_cond b e p : iProp Σ :=
-    (∀ a r, ⌜a ∈ₐ [[ b , e ]]⌝ → ▷ □ interp_expression r (WCap p b e a))%I.
+    (∀ a r i, ⌜a ∈ₐ [[ b , e ]]⌝ → ▷ □ interp_expression i r (WCap p b e a))%I.
 
   Lemma interp_exec_cond p b e a :
     p ≠ E -> interp (WCap p b e a) -∗ exec_cond b e p.
   Proof.
     iIntros (Hnp) "#Hw".
-    iIntros (a0 r Hin). iNext. iModIntro. 
+    iIntros (a0 i r Hin). iNext. iModIntro.
     iApply fundamental. 
     rewrite !fixpoint_interp1_eq /=. destruct p; try done.
   Qed.
@@ -173,57 +184,62 @@ Section fundamental.
   Lemma exec_wp p b e a :
     isCorrectPC (WCap p b e a) ->
     exec_cond b e p -∗
-    ∀ r, ▷ □ (interp_expr interp r) (WCap p b e a).
+    ∀ i r, ▷ □ (interp_expr interp r) i (WCap p b e a).
   Proof. 
     iIntros (Hvpc) "#Hexec". 
     rewrite /exec_cond.
-    iIntros (r). 
+    iIntros (i r).
     assert (a ∈ₐ[[b,e]])%I as Hin. 
     { rewrite /in_range. inversion Hvpc; subst. auto. }
-    iSpecialize ("Hexec" $! a r Hin). iFrame "#". 
+    iSpecialize ("Hexec" $! a i r Hin). iFrame "#".
   Qed.
 
   (* updatePcPerm adds a later because of the case of E-capabilities, which
      unfold to ▷ interp_expr *)
   Lemma interp_updatePcPerm w :
-    ⊢ interp w -∗ ▷ (∀ r, interp_expression r (updatePcPerm w)).
+    ⊢ interp w -∗ ▷ (∀ i r, interp_expression i r (updatePcPerm w)).
   Proof.
     iIntros "#Hw".
     assert ((∃ b e a, w = WCap E b e a) ∨ updatePcPerm w = w) as [Hw | ->].
     { destruct w; eauto. unfold updatePcPerm.
       case_match; eauto. }
     { destruct Hw as [b [e [a ->] ] ]. rewrite fixpoint_interp1_eq. cbn -[all_registers_s].
-      iNext. iIntros (rmap). iSpecialize ("Hw" $! rmap). iDestruct "Hw" as "#Hw".
-      iIntros "(HPC & Hr & ?)". iApply "Hw". iFrame. }
-    { iNext. iIntros (rmap). iApply fundamental. eauto. }
+      iNext. iIntros (i rmap). iSpecialize ("Hw" $! i rmap). iDestruct "Hw" as "#Hw".
+      iIntros "(HPC & Hr)". iApply "Hw". iFrame. }
+    { iNext. iIntros (rmap i). iApply fundamental. eauto. }
   Qed.
 
   Lemma jmp_to_unknown w :
     ⊢ interp w -∗
-      ▷ (∀ rmap,
-          ⌜dom (gset RegName) rmap = all_registers_s ∖ {[ PC ]}⌝ →
-          PC ↦ᵣ updatePcPerm w
+      ▷ (∀ (i: CoreN) rmap,
+          ⌜dom (gset (CoreN*RegName)) rmap = (set_map (fun r=> (i,r)) all_registers_s) ∖ {[ (i, PC) ]}⌝ →
+          (i, PC) ↦ᵣ updatePcPerm w
           ∗ ([∗ map] r↦w ∈ rmap, r ↦ᵣ w ∗ interp w)
-          ∗ na_own logrel_nais ⊤
-          -∗ WP Seq (Instr Executable) {{ λ v, ⌜v = HaltedV⌝ →
-               ∃ r : Reg, full_map r ∧ registers_mapsto r ∗ na_own logrel_nais ⊤ }}).
+          -∗ WP (i, Seq (Instr Executable)) {{ λ v, ⌜v = (i, HaltedV)⌝ →
+               ∃ r : Reg, full_map r i ∧ registers_mapsto r }}).
   Proof.
     iIntros "#Hw". iDestruct (interp_updatePcPerm with "Hw") as "Hw'". iNext.
-    iIntros (rmap Hrmap).
-    set rmap' := <[ PC := (WInt 0%Z: Word) ]> rmap : gmap RegName Word.
+    iIntros (i rmap Hrmap).
+    set rmap' := <[ (i, PC) := (WInt 0%Z: Word) ]> rmap
+        : gmap (CoreN*RegName) Word.
     iSpecialize ("Hw'" $! rmap').
-    iIntros "(HPC & Hr & Hna)". unfold interp_expression, interp_expr, interp_conf. cbn.
+    iIntros "(HPC & Hr)". unfold interp_expression, interp_expr, interp_conf. cbn.
     iApply "Hw'". iClear "Hw'". iFrame. rewrite /registers_mapsto.
     iDestruct (big_sepM_sep with "Hr") as "(Hr & HrV)".
     iSplitL "HrV"; [iSplit|].
-    { unfold full_map. iIntros (r).
-      destruct (decide (r = PC)). { subst r. rewrite lookup_insert //. eauto. }
-      rewrite lookup_insert_ne //. iPureIntro. rewrite elem_of_gmap_dom Hrmap. set_solver. }
-    { iIntros (ri v Hri Hvs).
-      rewrite lookup_insert_ne // in Hvs.
-      iDestruct (big_sepM_lookup _ _ ri with "HrV") as "HrV"; eauto. }
+    { unfold full_map. iIntros (r). 
+      destruct (decide (r = PC)).
+      { subst r. rewrite lookup_insert. iPureIntro. eauto. }
+      rewrite lookup_insert_ne;[| clear Hrmap; simplify_pair_eq].
+      iPureIntro. rewrite elem_of_gmap_dom Hrmap.
+      clear Hrmap; set_solver. }
+    { iIntros (j ri v Hri Hvs).
+      rewrite lookup_insert_ne in Hvs;[| clear Hrmap; simplify_pair_eq].
+      iDestruct (big_sepM_lookup _ _ (j, ri) with "HrV") as "HrV"; eauto.
+    }
     rewrite insert_insert. iApply big_sepM_insert.
-    { apply elem_of_gmap_dom_none. rewrite Hrmap. set_solver. }
+    { apply elem_of_gmap_dom_none. rewrite Hrmap ; clear Hrmap.
+      set_solver. }
     iFrame.
   Qed.
 
@@ -236,8 +252,8 @@ Section fundamental.
     { (* O *) rewrite fixpoint_interp1_eq //=. }
     4: { (* E *) rewrite fixpoint_interp1_eq /=.
          iDestruct (region_integers_alloc _ _ _ a _ RX with "H") as ">#H"; auto.
-         iModIntro. iIntros (r).
-         iDestruct (fundamental _ r with "H") as "H'". eauto. }
+         iModIntro. iIntros (r i).
+         iDestruct (fundamental r _ i with "H") as "H'". eauto. }
     all: iApply region_integers_alloc; eauto.
   Qed.
 
